veric/juicy_base.v
@@ -1,9 +1,6 @@
 Require Export VST.veric.base.
 Require Export VST.veric.res_predicates.
 
-(* patch for compcert maps notation conflict *)
-Global Notation "a ! b" := (Maps.PTree.get b a) (at level 1).
-
 (* Module Mem : MEM := compcert.common.Memory.Mem. *)
 Export Mem.
 Open Scope Z.
